\documentclass[12 pt]{article}
\pagestyle{empty}
\addtolength{\topmargin}{-0.9in}
\addtolength{\textheight}{1.9in}
\addtolength{\oddsidemargin}{-0.7in}
\addtolength{\textwidth}{1.4in}
\newcommand{\D}{\displaystyle}
\usepackage{amsmath}

\begin{document}
	\begin{center}
		\textbf{\hfill Math 226/229 -- Quiz} \\
	\end{center}
	\medskip

	\noindent
	\textbf{Week 4 Quiz Solutions.} \hfill
	\vspace{.1in}
	%\textbf{Discussion: 10 am   11 am}\
	\hspace*{0.2in}
	\medskip
	\noindent
	\begin{enumerate}
		\item (\textit{5 points})
    Find a parametric equation of the line through the point $(1, 2, -1)$ and
    perpendicular to both $\mathbf{i} + \mathbf{j}$ and
    $\mathbf{j} - 2\mathbf{k}$.
		\\~\\
    \textbf{Solution.}
		\\
		The parametric equation of a line through $(x_0, y_0, z_0)$ parallel to
		$\langle a, b, c\rangle$ is given by the parametric equations \begin{align*}
			x &= x_0 + at \\
			y &= y_0 + bt \\
			z &= z_0 + ct.
		\end{align*}
		We can find a vector $\langle a, b, c \rangle$ perpendicular to both
		$\mathbf{i} + \mathbf{j}$ and $\mathbf{j} - 2\mathbf{k}$ by taking the cross
		product. \[
			\begin{vmatrix}
				\mathbf i & \mathbf j & \mathbf k \\
				1 & 1 & 0 \\
				0 & 1 & -2
			\end{vmatrix}
			= \mathbf i \begin{vmatrix} 1 & 0 \\ 1 & -2 \end{vmatrix}
			- \mathbf j \begin{vmatrix} 1 & 0 \\ 0 & -2 \end{vmatrix}
			+ \mathbf k \begin{vmatrix} 1 & 1 \\ 0 & 1 \end{vmatrix}
			= -2\mathbf i + 2\mathbf j + \mathbf k
		\]
		Therefore (one choice for) the desired parametric equations is \begin{align*}
			x &= 1 - 2t \\
			y &= 2 + 2t \\
			z &= -1 + t.
		\end{align*}
		\item (\textit{5 points})
		Find the equation of the plane through the point $(2, 2, 9)$ and
		perpendicular to the line $x = 2t$, $y = 1 + 2t$, and $z = 4 - t$.
		\\~\\
		\textbf{Solution.}
		The paramteric equations described a line that is parallel to the vector
		$\langle 2, 2, -1 \rangle$. Thus the desired plane is of the form \[
			2x + 2y - z + d = 0.
		\] Choosing our point on the plane, $(x, y, z) = (2, 2, 9)$, allows us to
		solve for $d$ \begin{align*}
			2(2) + 2(2) - 9 + d &= 0 \\
			d &= 1.
		\end{align*} So the desired equation is \[
			2x + 2y - z + 1 = 0.
		\]
  \end{enumerate}
\end{document}
