\documentclass{article}

\usepackage[margin=1in]{geometry}
\usepackage{amsmath,amsthm,amssymb}
\usepackage{bbm, enumerate, tikz}
\usepackage{multicol}

\newenvironment{problem}[2][Problem]{\begin{trivlist}
\item[\hskip \labelsep {\bfseries #1}\hskip \labelsep {\bfseries #2.}]}{\end{trivlist}}
\newenvironment{solution}[1][Solution.]{\begin{trivlist}
\item[\hskip \labelsep {\bfseries #1}]}{\end{trivlist}}

\begin{document}

\title{Problem 5 solutions.}
% \author{Peter Kagey}
\date{}

\maketitle

% -----------------------------------------------------
% First problem
% -----------------------------------------------------
\begin{problem}{1}
  Evaluate the integral \[
    \int(3x^2 - 1)\ln(x)\, dx.
  \]
\end{problem}

\begin{solution} $ $\\
  We'll use integration by parts. Let \begin{align*}
    u = \ln(x)  &\hspace{0.5cm} du = \frac{1}{x}\,dx \\
    v = x^3 - x &\hspace{0.5cm} dv = 3x^2 - 1 \,dx.
  \end{align*}
  Then \begin{align*}
    \int(3x^2 - 1)\ln(x)\, dx
    &= (x^3 - x)\ln(x) - \int \frac{x^3 - x}{x}\, dx \\
    &= (x^3 - x)\ln(x) - \int x^2 - 1\, dx \\
    &= (x^3 - x)\ln(x) - \frac{x^3}{3} - x + c
  \end{align*}
\end{solution}
% -----------------------------------------------------
% Second problem
% -----------------------------------------------------
\begin{problem}{2}
  Evaluate the integral \[
    \int_1^2 \frac{1}{4+x^2}\,dx
  \]
\end{problem}

\begin{solution} $ $\\
  We'll use the identity \[
    \frac{d}{dx}\arctan(x) = \frac{1}{1+x^2}.
  \]

  Begin by dividing the denominator by $4$, \[
    \int_1^2 \frac{1}{4+x^2}\,dx = \frac{1}{4} \int_1^2 \frac{1}{1+x^2/4}\,dx
  \]
  Then substituting $u = x/2$ and $du = dx/2$ gives \[
    \int_1^2 \frac{1}{4+x^2}\,dx
    = \frac{2}{4}\int_{u=1/2}^1 \frac{1}{1+u^2}\,du
    = \left[\frac{1}{2}\arctan(u)\right]_{1/2}^1
    = \frac{\pi}{8} - \frac{\arctan(\frac{1}{2})}{2}
  \]
\end{solution}

% -----------------------------------------------------
% Third problem
% -----------------------------------------------------
\pagebreak
\begin{problem}{3}
  Evaluate the integral \[
    \int \arcsin(x)\,dx
  \]
\end{problem}

\begin{solution} $ $\\
  We'll use integration by parts. Let \begin{align*}
    u = \arcsin(x)  &\hspace{0.5cm} du = \frac{1}{\sqrt{1 - x^2}}\,dx \\
    v = x &\hspace{0.5cm} dv = dx.
  \end{align*}
  Then \begin{align*}
    \int \arcsin(x)\,dx = x\arcsin(x) - \int \frac{x}{\sqrt{1 - x^2}}\,dx
  \end{align*}
  Substituting $u = 1 - x^2$ and $du = -2x\,dx$ gives \[
    \int \frac{x}{\sqrt{1 - x^2}}\,dx
    = -\frac{1}{2}\int \frac{du}{\sqrt{u}}
    = -\sqrt{u} + c
    = -\sqrt{1 - x^2} + c
  \]
  Thus the original integral becomes \[
    \int \arcsin(x)\,dx = x\arcsin(x) + \sqrt{1 - x^2} + c
  \]
\end{solution}

% -----------------------------------------------------
% Fourth problem
% -----------------------------------------------------
\begin{problem}{4}
  Evaluate the integral \[
    \int \sin(\sqrt{y})\,dy
  \]
\end{problem}

\begin{solution} $ $\\
  This is a tricky substitution. Let \begin{align*}
    u = \sqrt{y} \text{\ \ and\ \ } du = \frac{1}{2\sqrt{y}}\,dy.
  \end{align*}
  Now solving for $dy$ gives \[
    2\underbrace{\sqrt{y}}_udu = dy = 2u\,du.
  \]
  Plugging this in gives \begin{align*}
    \int \sin(\sqrt{y})\,dy &= 2\int u\sin(u)\, du.
  \end{align*}
  And now using integration by parts with \begin{align*}
    w = u  &\hspace{0.5cm} dw = du \\
    v = -\cos(u) &\hspace{0.5cm} dv = \sin(u) \,du
  \end{align*}
  gives \begin{align*}
    2\int u\sin(u)\, du &= 2\left(-u\cos(u) + \int\cos(u)\, du\right) \\
    &= 2\sin(u) -2u\cos(u) + c\\
    &= 2\sin(\sqrt{y}) -2\sqrt{y}\cos(\sqrt{y}) + c
  \end{align*}
\end{solution}

% -----------------------------------------------------
% Fifth problem
% -----------------------------------------------------
\pagebreak
\begin{problem}{5}
  Evaluate the integral \[
    \int e^{2x}\sin(x)\,dx.
  \]
\end{problem}

\begin{solution} $ $\\
  Here we do repeated integration by parts.
  First let \begin{align*}
    u = e^{2x}  &\hspace{0.5cm} du = 2e^{2x}\,dx \\
    v = -\cos(x) &\hspace{0.5cm} dv = \sin(x) \,dx.
  \end{align*} Then \[
    \int e^{2x}\sin(x)\,dx = -\cos(x)e^{2x} + 2\int \cos(x)e^{2x}\,dx.
  \]
  Next use \begin{align*}
    u = e^{2x}  &\hspace{0.5cm} du = 2e^{2x}\,dx \\
    v = \sin(x) &\hspace{0.5cm} dv = \cos(x) \,dx.
  \end{align*}
  This gives \begin{align*}
    \int e^{2x}\sin(x)\,dx
    &= -\cos(x)e^{2x} + 2\left(\sin(x)e^{2x} - 2\int \sin(x)e^{2x}\,dx\right)\\
    &= -\cos(x)e^{2x} + 2\sin(x)e^{2x} - 4\int e^{2x}\sin(x)\,dx.
  \end{align*}
  Solving for our original integral gives \[
    \int e^{2x}\sin(x)\,dx = \frac{1}{5}\left(2\sin(x)e^{2x}-\cos(x)e^{2x}\right).
  \]

\end{solution}

% -----------------------------------------------------
% Sixth problem
% -----------------------------------------------------
\begin{problem}{6}
  Evaluate the integral \[
    \int_0^5 2x + \sqrt{25 - x^2}\,dx.
  \]
\end{problem}

\begin{solution} $ $\\
  This is best solved geometrically. The fuction $\sqrt{25 - x^2}$ describes the
  semicircle above the $x$-axis of radius $5$, so integrating from $0$ to $5$
  gives the area of quarter circle of radius $5$, $25\pi/4$.\\
  The other integral is quick: \[
    \int_0^5 2x\,dx = [x^2]_0^5 = 25.
  \]
  Thus \[
    \int_0^5 2x + \sqrt{25 - x^2}\,dx = \frac{25\pi}{4} + 25.
  \]

\end{solution}

% -----------------------------------------------------
% Seventh problem
% -----------------------------------------------------
\pagebreak
\begin{problem}{7}
  Evaluate the integral \[
    \int_0^1 \frac{x^3}{\sqrt{2 + x^2}}\,dx.
  \]
\end{problem}

\begin{solution} $ $\\
  This requires a substitution similar in spirit to problem 5.4.
  Let $u = 2 + x^2$ and $du = 2x\,dx$. Then $x^2 = u - 2$, so we can rewrite the
  integral as \begin{align*}
    \frac{1}{2}\int_{u=2}^3 \frac{u - 2}{\sqrt{u}}\,du
    &= \frac{1}{2}\int_2^3 \sqrt{u} - \frac{2}{\sqrt{u}}\,du \\
    &= \frac{1}{2}\left[\frac{2}{3}u^{3/2} - 4u^{1/2}\right]_2^3 \\
    &= \sqrt{3} - 2\sqrt{3} - \frac{2}{3}\sqrt{2} + 2\sqrt{2} \\
    &=  \frac{4}{3}\sqrt{2} - \sqrt{3}
  \end{align*}
\end{solution}

% -----------------------------------------------------
% Eighth problem
% -----------------------------------------------------
\begin{problem}{8}
  Evaluate the integral \[
    \int_{-1}^1 x^3e^{x^2 + 1}\, dx.
  \]
\end{problem}

\begin{solution} $ $\\
  We can use the same trick as before. Let $u = x^2 + 1$ and $du = 2x\, dx$.
  This means that $x^2 = u - 1$. So \[
    \frac{1}{2}\int_{u=2}^2 (u - 1)e^u\, du = 0.
  \] based on the bounds of integration.\\
  (It is enough to check that the original integrand is odd.)
\end{solution}

\end{document}
